src/HOL/Auth/Yahalom2.thy
@@ -26,33 +26,33 @@ inductive_set yahalom :: "event list set"
          (*The spy MAY say anything he CAN say.  We do not expect him to
            invent new nonces here, but he can also use NS1.  Common to
            all similar protocols.*)
- | Fake: "[| evsf \<in> yahalom;  X \<in> synth (analz (knows Spy evsf)) |]
-          ==> Says Spy B X  # evsf \<in> yahalom"
+ | Fake: "\<lbrakk>evsf \<in> yahalom;  X \<in> synth (analz (knows Spy evsf))\<rbrakk>
+          \<Longrightarrow> Says Spy B X  # evsf \<in> yahalom"
 
          (*A message that has been sent can be received by the
            intended recipient.*)
- | Reception: "[| evsr \<in> yahalom;  Says A B X \<in> set evsr |]
-               ==> Gets B X # evsr \<in> yahalom"
+ | Reception: "\<lbrakk>evsr \<in> yahalom;  Says A B X \<in> set evsr\<rbrakk>
+               \<Longrightarrow> Gets B X # evsr \<in> yahalom"
 
          (*Alice initiates a protocol run*)
- | YM1:  "[| evs1 \<in> yahalom;  Nonce NA \<notin> used evs1 |]
-          ==> Says A B \<lbrace>Agent A, Nonce NA\<rbrace> # evs1 \<in> yahalom"
+ | YM1:  "\<lbrakk>evs1 \<in> yahalom;  Nonce NA \<notin> used evs1\<rbrakk>
+          \<Longrightarrow> Says A B \<lbrace>Agent A, Nonce NA\<rbrace> # evs1 \<in> yahalom"
 
          (*Bob's response to Alice's message.*)
- | YM2:  "[| evs2 \<in> yahalom;  Nonce NB \<notin> used evs2;
-             Gets B \<lbrace>Agent A, Nonce NA\<rbrace> \<in> set evs2 |]
-          ==> Says B Server
+ | YM2:  "\<lbrakk>evs2 \<in> yahalom;  Nonce NB \<notin> used evs2;
+             Gets B \<lbrace>Agent A, Nonce NA\<rbrace> \<in> set evs2\<rbrakk>
+          \<Longrightarrow> Says B Server
                   \<lbrace>Agent B, Nonce NB, Crypt (shrK B) \<lbrace>Agent A, Nonce NA\<rbrace>\<rbrace>
                 # evs2 \<in> yahalom"
 
          (*The Server receives Bob's message.  He responds by sending a
            new session key to Alice, with a certificate for forwarding to Bob.
            Both agents are quoted in the 2nd certificate to prevent attacks!*)
- | YM3:  "[| evs3 \<in> yahalom;  Key KAB \<notin> used evs3;
+ | YM3:  "\<lbrakk>evs3 \<in> yahalom;  Key KAB \<notin> used evs3;
              Gets Server \<lbrace>Agent B, Nonce NB,
                            Crypt (shrK B) \<lbrace>Agent A, Nonce NA\<rbrace>\<rbrace>
-               \<in> set evs3 |]
-          ==> Says Server A
+               \<in> set evs3\<rbrakk>
+          \<Longrightarrow> Says Server A
                \<lbrace>Nonce NB,
                  Crypt (shrK A) \<lbrace>Agent B, Key KAB, Nonce NA\<rbrace>,
                  Crypt (shrK B) \<lbrace>Agent A, Agent B, Key KAB, Nonce NB\<rbrace>\<rbrace>
@@ -60,20 +60,20 @@ inductive_set yahalom :: "event list set"
 
          (*Alice receives the Server's (?) message, checks her Nonce, and
            uses the new session key to send Bob his Nonce.*)
- | YM4:  "[| evs4 \<in> yahalom;
+ | YM4:  "\<lbrakk>evs4 \<in> yahalom;
              Gets A \<lbrace>Nonce NB, Crypt (shrK A) \<lbrace>Agent B, Key K, Nonce NA\<rbrace>,
                       X\<rbrace>  \<in> set evs4;
-             Says A B \<lbrace>Agent A, Nonce NA\<rbrace> \<in> set evs4 |]
-          ==> Says A B \<lbrace>X, Crypt K (Nonce NB)\<rbrace> # evs4 \<in> yahalom"
+             Says A B \<lbrace>Agent A, Nonce NA\<rbrace> \<in> set evs4\<rbrakk>
+          \<Longrightarrow> Says A B \<lbrace>X, Crypt K (Nonce NB)\<rbrace> # evs4 \<in> yahalom"
 
          (*This message models possible leaks of session keys.  The nonces
            identify the protocol run.  Quoting Server here ensures they are
            correct. *)
- | Oops: "[| evso \<in> yahalom;
+ | Oops: "\<lbrakk>evso \<in> yahalom;
              Says Server A \<lbrace>Nonce NB,
                              Crypt (shrK A) \<lbrace>Agent B, Key K, Nonce NA\<rbrace>,
-                             X\<rbrace>  \<in> set evso |]
-          ==> Notes Spy \<lbrace>Nonce NA, Nonce NB, Key K\<rbrace> # evso \<in> yahalom"
+                             X\<rbrace>  \<in> set evso\<rbrakk>
+          \<Longrightarrow> Notes Spy \<lbrace>Nonce NA, Nonce NB, Key K\<rbrace> # evso \<in> yahalom"
 
 
 declare Says_imp_knows_Spy [THEN analz.Inj, dest]
@@ -83,7 +83,7 @@ declare analz_into_parts [dest]
 
 text\<open>A "possibility property": there are traces that reach the end\<close>
 lemma "Key K \<notin> used []
-       ==> \<exists>X NB. \<exists>evs \<in> yahalom.
+       \<Longrightarrow> \<exists>X NB. \<exists>evs \<in> yahalom.
              Says A B \<lbrace>X, Crypt K (Nonce NB)\<rbrace> \<in> set evs"
 apply (intro exI bexI)
 apply (rule_tac [2] yahalom.Nil
@@ -95,12 +95,12 @@ apply (possibility, simp add: used_Cons)
 done
 
 lemma Gets_imp_Says:
-     "[| Gets B X \<in> set evs; evs \<in> yahalom |] ==> \<exists>A. Says A B X \<in> set evs"
+     "\<lbrakk>Gets B X \<in> set evs; evs \<in> yahalom\<rbrakk> \<Longrightarrow> \<exists>A. Says A B X \<in> set evs"
 by (erule rev_mp, erule yahalom.induct, auto)
 
 text\<open>Must be proved separately for each protocol\<close>
 lemma Gets_imp_knows_Spy:
-     "[| Gets B X \<in> set evs; evs \<in> yahalom |]  ==> X \<in> knows Spy evs"
+     "\<lbrakk>Gets B X \<in> set evs; evs \<in> yahalom\<rbrakk>  \<Longrightarrow> X \<in> knows Spy evs"
 by (blast dest!: Gets_imp_Says Says_imp_knows_Spy)
 
 declare Gets_imp_knows_Spy [THEN analz.Inj, dest]
@@ -111,8 +111,8 @@ subsection\<open>Inductive Proofs\<close>
 text\<open>Result for reasoning about the encrypted portion of messages.
 Lets us treat YM4 using a similar argument as for the Fake case.\<close>
 lemma YM4_analz_knows_Spy:
-     "[| Gets A \<lbrace>NB, Crypt (shrK A) Y, X\<rbrace> \<in> set evs;  evs \<in> yahalom |]
-      ==> X \<in> analz (knows Spy evs)"
+     "\<lbrakk>Gets A \<lbrace>NB, Crypt (shrK A) Y, X\<rbrace> \<in> set evs;  evs \<in> yahalom\<rbrakk>
+      \<Longrightarrow> X \<in> analz (knows Spy evs)"
 by blast
 
 lemmas YM4_parts_knows_Spy =
@@ -124,49 +124,45 @@ lemmas YM4_parts_knows_Spy =
 
 text\<open>Spy never sees a good agent's shared key!\<close>
 lemma Spy_see_shrK [simp]:
-     "evs \<in> yahalom ==> (Key (shrK A) \<in> parts (knows Spy evs)) = (A \<in> bad)"
+     "evs \<in> yahalom \<Longrightarrow> (Key (shrK A) \<in> parts (knows Spy evs)) = (A \<in> bad)"
 by (erule yahalom.induct, force,
     drule_tac [6] YM4_parts_knows_Spy, simp_all, blast+)
 
 lemma Spy_analz_shrK [simp]:
-     "evs \<in> yahalom ==> (Key (shrK A) \<in> analz (knows Spy evs)) = (A \<in> bad)"
+     "evs \<in> yahalom \<Longrightarrow> (Key (shrK A) \<in> analz (knows Spy evs)) = (A \<in> bad)"
 by auto
 
 lemma Spy_see_shrK_D [dest!]:
-     "[|Key (shrK A) \<in> parts (knows Spy evs);  evs \<in> yahalom|] ==> A \<in> bad"
+     "\<lbrakk>Key (shrK A) \<in> parts (knows Spy evs);  evs \<in> yahalom\<rbrakk> \<Longrightarrow> A \<in> bad"
 by (blast dest: Spy_see_shrK)
 
 text\<open>Nobody can have used non-existent keys!  
     Needed to apply \<open>analz_insert_Key\<close>\<close>
 lemma new_keys_not_used [simp]:
-    "[|Key K \<notin> used evs; K \<in> symKeys; evs \<in> yahalom|]
-     ==> K \<notin> keysFor (parts (spies evs))"
+    "\<lbrakk>Key K \<notin> used evs; K \<in> symKeys; evs \<in> yahalom\<rbrakk>
+     \<Longrightarrow> K \<notin> keysFor (parts (spies evs))"
 apply (erule rev_mp)
 apply (erule yahalom.induct, force,
        frule_tac [6] YM4_parts_knows_Spy, simp_all)
-txt\<open>Fake\<close>
-apply (force dest!: keysFor_parts_insert)
-txt\<open>YM3\<close>
-apply blast
-txt\<open>YM4\<close>
-apply auto
-apply (blast dest!: Gets_imp_knows_Spy [THEN parts.Inj])
+subgoal --\<open>Fake\<close> by (force dest!: keysFor_parts_insert)
+subgoal --\<open>YM3 \<close>by blast
+subgoal --\<open>YM4\<close> by (fastforce dest!: Gets_imp_knows_Spy [THEN parts.Inj])
 done
 
 
 text\<open>Describes the form of K when the Server sends this message.  Useful for
   Oops as well as main secrecy property.\<close>
 lemma Says_Server_message_form:
-     "[| Says Server A \<lbrace>nb', Crypt (shrK A) \<lbrace>Agent B, Key K, na\<rbrace>, X\<rbrace>
-          \<in> set evs;  evs \<in> yahalom |]
-      ==> K \<notin> range shrK"
+     "\<lbrakk>Says Server A \<lbrace>nb', Crypt (shrK A) \<lbrace>Agent B, Key K, na\<rbrace>, X\<rbrace>
+          \<in> set evs;  evs \<in> yahalom\<rbrakk>
+      \<Longrightarrow> K \<notin> range shrK"
 by (erule rev_mp, erule yahalom.induct, simp_all)
 
 
 (****
  The following is to prove theorems of the form
 
-          Key K \<in> analz (insert (Key KAB) (knows Spy evs)) ==>
+          Key K \<in> analz (insert (Key KAB) (knows Spy evs)) \<Longrightarrow>
           Key K \<in> analz (knows Spy evs)
 
  A more general formula must be proved inductively.
@@ -175,7 +171,7 @@ by (erule rev_mp, erule yahalom.induct, simp_all)
 (** Session keys are not used to encrypt other session keys **)
 
 lemma analz_image_freshK [rule_format]:
- "evs \<in> yahalom ==>
+ "evs \<in> yahalom \<Longrightarrow>
    \<forall>K KK. KK <= - (range shrK) -->
           (Key K \<in> analz (Key`KK Un (knows Spy evs))) =
           (K \<in> KK | Key K \<in> analz (knows Spy evs))"
@@ -185,7 +181,7 @@ apply (drule_tac [7] YM4_analz_knows_Spy, analz_freshK, spy_analz, blast)
 done
 
 lemma analz_insert_freshK:
-     "[| evs \<in> yahalom;  KAB \<notin> range shrK |] ==>
+     "\<lbrakk>evs \<in> yahalom;  KAB \<notin> range shrK\<rbrakk> \<Longrightarrow>
       (Key K \<in> analz (insert (Key KAB) (knows Spy evs))) =
       (K = KAB | Key K \<in> analz (knows Spy evs))"
 by (simp only: analz_image_freshK analz_image_freshK_simps)
@@ -193,12 +189,12 @@ by (simp only: analz_image_freshK analz_image_freshK_simps)
 
 text\<open>The Key K uniquely identifies the Server's  message\<close>
 lemma unique_session_keys:
-     "[| Says Server A
+     "\<lbrakk>Says Server A
           \<lbrace>nb, Crypt (shrK A) \<lbrace>Agent B, Key K, na\<rbrace>, X\<rbrace> \<in> set evs;
         Says Server A'
           \<lbrace>nb', Crypt (shrK A') \<lbrace>Agent B', Key K, na'\<rbrace>, X'\<rbrace> \<in> set evs;
-        evs \<in> yahalom |]
-     ==> A=A' & B=B' & na=na' & nb=nb'"
+        evs \<in> yahalom\<rbrakk>
+     \<Longrightarrow> A=A' & B=B' & na=na' & nb=nb'"
 apply (erule rev_mp, erule rev_mp)
 apply (erule yahalom.induct, simp_all)
 txt\<open>YM3, by freshness\<close>
@@ -209,8 +205,8 @@ done
 subsection\<open>Crucial Secrecy Property: Spy Does Not See Key @{term KAB}\<close>
 
 lemma secrecy_lemma:
-     "[| A \<notin> bad;  B \<notin> bad;  evs \<in> yahalom |]
-      ==> Says Server A
+     "\<lbrakk>A \<notin> bad;  B \<notin> bad;  evs \<in> yahalom\<rbrakk>
+      \<Longrightarrow> Says Server A
             \<lbrace>nb, Crypt (shrK A) \<lbrace>Agent B, Key K, na\<rbrace>,
                   Crypt (shrK B) \<lbrace>Agent A, Agent B, Key K, nb\<rbrace>\<rbrace>
            \<in> set evs -->
@@ -225,13 +221,13 @@ done
 
 text\<open>Final version\<close>
 lemma Spy_not_see_encrypted_key:
-     "[| Says Server A
+     "\<lbrakk>Says Server A
             \<lbrace>nb, Crypt (shrK A) \<lbrace>Agent B, Key K, na\<rbrace>,
                   Crypt (shrK B) \<lbrace>Agent A, Agent B, Key K, nb\<rbrace>\<rbrace>
          \<in> set evs;
          Notes Spy \<lbrace>na, nb, Key K\<rbrace> \<notin> set evs;
-         A \<notin> bad;  B \<notin> bad;  evs \<in> yahalom |]
-      ==> Key K \<notin> analz (knows Spy evs)"
+         A \<notin> bad;  B \<notin> bad;  evs \<in> yahalom\<rbrakk>
+      \<Longrightarrow> Key K \<notin> analz (knows Spy evs)"
 by (blast dest: secrecy_lemma Says_Server_message_form)
 
 
@@ -244,13 +240,13 @@ to the previous result in that the Spy already has @{term analz} and
 other than Fake are trivial, while Fake requires
 @{term "Key K \<notin> analz (knows Spy evs)"}.\<close>
 lemma Spy_not_know_encrypted_key:
-     "[| Says Server A
+     "\<lbrakk>Says Server A
             \<lbrace>nb, Crypt (shrK A) \<lbrace>Agent B, Key K, na\<rbrace>,
                   Crypt (shrK B) \<lbrace>Agent A, Agent B, Key K, nb\<rbrace>\<rbrace>
          \<in> set evs;
          Notes Spy \<lbrace>na, nb, Key K\<rbrace> \<notin> set evs;
-         A \<notin> bad;  B \<notin> bad;  evs \<in> yahalom |]
-      ==> Key K \<notin> knows Spy evs"
+         A \<notin> bad;  B \<notin> bad;  evs \<in> yahalom\<rbrakk>
+      \<Longrightarrow> Key K \<notin> knows Spy evs"
 by (blast dest: Spy_not_see_encrypted_key)
 
 
@@ -259,9 +255,9 @@ subsection\<open>Security Guarantee for A upon receiving YM3\<close>
 text\<open>If the encrypted message appears then it originated with the Server.
   May now apply \<open>Spy_not_see_encrypted_key\<close>, subject to its conditions.\<close>
 lemma A_trusts_YM3:
-     "[| Crypt (shrK A) \<lbrace>Agent B, Key K, na\<rbrace> \<in> parts (knows Spy evs);
-         A \<notin> bad;  evs \<in> yahalom |]
-      ==> \<exists>nb. Says Server A
+     "\<lbrakk>Crypt (shrK A) \<lbrace>Agent B, Key K, na\<rbrace> \<in> parts (knows Spy evs);
+         A \<notin> bad;  evs \<in> yahalom\<rbrakk>
+      \<Longrightarrow> \<exists>nb. Says Server A
                     \<lbrace>nb, Crypt (shrK A) \<lbrace>Agent B, Key K, na\<rbrace>,
                           Crypt (shrK B) \<lbrace>Agent A, Agent B, Key K, nb\<rbrace>\<rbrace>
                   \<in> set evs"
@@ -275,10 +271,10 @@ done
 text\<open>The obvious combination of \<open>A_trusts_YM3\<close> with 
 \<open>Spy_not_see_encrypted_key\<close>\<close>
 theorem A_gets_good_key:
-     "[| Crypt (shrK A) \<lbrace>Agent B, Key K, na\<rbrace> \<in> parts (knows Spy evs);
+     "\<lbrakk>Crypt (shrK A) \<lbrace>Agent B, Key K, na\<rbrace> \<in> parts (knows Spy evs);
          \<forall>nb. Notes Spy \<lbrace>na, nb, Key K\<rbrace> \<notin> set evs;
-         A \<notin> bad;  B \<notin> bad;  evs \<in> yahalom |]
-      ==> Key K \<notin> analz (knows Spy evs)"
+         A \<notin> bad;  B \<notin> bad;  evs \<in> yahalom\<rbrakk>
+      \<Longrightarrow> Key K \<notin> analz (knows Spy evs)"
 by (blast dest!: A_trusts_YM3 Spy_not_see_encrypted_key)
 
 
@@ -287,10 +283,10 @@ subsection\<open>Security Guarantee for B upon receiving YM4\<close>
 text\<open>B knows, by the first part of A's message, that the Server distributed
   the key for A and B, and has associated it with NB.\<close>
 lemma B_trusts_YM4_shrK:
-     "[| Crypt (shrK B) \<lbrace>Agent A, Agent B, Key K, Nonce NB\<rbrace>
+     "\<lbrakk>Crypt (shrK B) \<lbrace>Agent A, Agent B, Key K, Nonce NB\<rbrace>
            \<in> parts (knows Spy evs);
-         B \<notin> bad;  evs \<in> yahalom |]
-  ==> \<exists>NA. Says Server A
+         B \<notin> bad;  evs \<in> yahalom\<rbrakk>
+  \<Longrightarrow> \<exists>NA. Says Server A
              \<lbrace>Nonce NB,
                Crypt (shrK A) \<lbrace>Agent B, Key K, Nonce NA\<rbrace>,
                Crypt (shrK B) \<lbrace>Agent A, Agent B, Key K, Nonce NB\<rbrace>\<rbrace>
@@ -309,10 +305,10 @@ text\<open>With this protocol variant, we don't need the 2nd part of YM4 at all:
 text\<open>What can B deduce from receipt of YM4?  Stronger and simpler than Yahalom
   because we do not have to show that NB is secret.\<close>
 lemma B_trusts_YM4:
-     "[| Gets B \<lbrace>Crypt (shrK B) \<lbrace>Agent A, Agent B, Key K, Nonce NB\<rbrace>,  X\<rbrace>
+     "\<lbrakk>Gets B \<lbrace>Crypt (shrK B) \<lbrace>Agent A, Agent B, Key K, Nonce NB\<rbrace>,  X\<rbrace>
            \<in> set evs;
-         A \<notin> bad;  B \<notin> bad;  evs \<in> yahalom |]
-  ==> \<exists>NA. Says Server A
+         A \<notin> bad;  B \<notin> bad;  evs \<in> yahalom\<rbrakk>
+  \<Longrightarrow> \<exists>NA. Says Server A
              \<lbrace>Nonce NB,
                Crypt (shrK A) \<lbrace>Agent B, Key K, Nonce NA\<rbrace>,
                Crypt (shrK B) \<lbrace>Agent A, Agent B, Key K, Nonce NB\<rbrace>\<rbrace>
@@ -323,11 +319,11 @@ by (blast dest!: B_trusts_YM4_shrK)
 text\<open>The obvious combination of \<open>B_trusts_YM4\<close> with 
 \<open>Spy_not_see_encrypted_key\<close>\<close>
 theorem B_gets_good_key:
-     "[| Gets B \<lbrace>Crypt (shrK B) \<lbrace>Agent A, Agent B, Key K, Nonce NB\<rbrace>, X\<rbrace>
+     "\<lbrakk>Gets B \<lbrace>Crypt (shrK B) \<lbrace>Agent A, Agent B, Key K, Nonce NB\<rbrace>, X\<rbrace>
            \<in> set evs;
          \<forall>na. Notes Spy \<lbrace>na, Nonce NB, Key K\<rbrace> \<notin> set evs;
-         A \<notin> bad;  B \<notin> bad;  evs \<in> yahalom |]
-      ==> Key K \<notin> analz (knows Spy evs)"
+         A \<notin> bad;  B \<notin> bad;  evs \<in> yahalom\<rbrakk>
+      \<Longrightarrow> Key K \<notin> analz (knows Spy evs)"
 by (blast dest!: B_trusts_YM4 Spy_not_see_encrypted_key)
 
 
@@ -335,9 +331,9 @@ subsection\<open>Authenticating B to A\<close>
 
 text\<open>The encryption in message YM2 tells us it cannot be faked.\<close>
 lemma B_Said_YM2:
-     "[| Crypt (shrK B) \<lbrace>Agent A, Nonce NA\<rbrace> \<in> parts (knows Spy evs);
-         B \<notin> bad;  evs \<in> yahalom |]
-      ==> \<exists>NB. Says B Server \<lbrace>Agent B, Nonce NB,
+     "\<lbrakk>Crypt (shrK B) \<lbrace>Agent A, Nonce NA\<rbrace> \<in> parts (knows Spy evs);
+         B \<notin> bad;  evs \<in> yahalom\<rbrakk>
+      \<Longrightarrow> \<exists>NB. Says B Server \<lbrace>Agent B, Nonce NB,
                                Crypt (shrK B) \<lbrace>Agent A, Nonce NA\<rbrace>\<rbrace>
                       \<in> set evs"
 apply (erule rev_mp)
@@ -350,10 +346,10 @@ done
 
 text\<open>If the server sends YM3 then B sent YM2, perhaps with a different NB\<close>
 lemma YM3_auth_B_to_A_lemma:
-     "[| Says Server A \<lbrace>nb, Crypt (shrK A) \<lbrace>Agent B, Key K, Nonce NA\<rbrace>, X\<rbrace>
+     "\<lbrakk>Says Server A \<lbrace>nb, Crypt (shrK A) \<lbrace>Agent B, Key K, Nonce NA\<rbrace>, X\<rbrace>
            \<in> set evs;
-         B \<notin> bad;  evs \<in> yahalom |]
-      ==> \<exists>nb'. Says B Server \<lbrace>Agent B, nb',
+         B \<notin> bad;  evs \<in> yahalom\<rbrakk>
+      \<Longrightarrow> \<exists>nb'. Says B Server \<lbrace>Agent B, nb',
                                    Crypt (shrK B) \<lbrace>Agent A, Nonce NA\<rbrace>\<rbrace>
                        \<in> set evs"
 apply (erule rev_mp)
@@ -364,10 +360,10 @@ done
 
 text\<open>If A receives YM3 then B has used nonce NA (and therefore is alive)\<close>
 theorem YM3_auth_B_to_A:
-     "[| Gets A \<lbrace>nb, Crypt (shrK A) \<lbrace>Agent B, Key K, Nonce NA\<rbrace>, X\<rbrace>
+     "\<lbrakk>Gets A \<lbrace>nb, Crypt (shrK A) \<lbrace>Agent B, Key K, Nonce NA\<rbrace>, X\<rbrace>
            \<in> set evs;
-         A \<notin> bad;  B \<notin> bad;  evs \<in> yahalom |]
- ==> \<exists>nb'. Says B Server
+         A \<notin> bad;  B \<notin> bad;  evs \<in> yahalom\<rbrakk>
+ \<Longrightarrow> \<exists>nb'. Says B Server
                   \<lbrace>Agent B, nb', Crypt (shrK B) \<lbrace>Agent A, Nonce NA\<rbrace>\<rbrace>
                \<in> set evs"
 by (blast dest!: A_trusts_YM3 YM3_auth_B_to_A_lemma)
@@ -385,16 +381,16 @@ text\<open>Assuming the session key is secure, if both certificates are present 
 text\<open>This lemma allows a use of \<open>unique_session_keys\<close> in the next proof,
   which otherwise is extremely slow.\<close>
 lemma secure_unique_session_keys:
-     "[| Crypt (shrK A) \<lbrace>Agent B, Key K, na\<rbrace> \<in> analz (spies evs);
+     "\<lbrakk>Crypt (shrK A) \<lbrace>Agent B, Key K, na\<rbrace> \<in> analz (spies evs);
          Crypt (shrK A') \<lbrace>Agent B', Key K, na'\<rbrace> \<in> analz (spies evs);
-         Key K \<notin> analz (knows Spy evs);  evs \<in> yahalom |]
-     ==> A=A' & B=B'"
+         Key K \<notin> analz (knows Spy evs);  evs \<in> yahalom\<rbrakk>
+     \<Longrightarrow> A=A' & B=B'"
 by (blast dest!: A_trusts_YM3 dest: unique_session_keys Crypt_Spy_analz_bad)
 
 
 lemma Auth_A_to_B_lemma [rule_format]:
      "evs \<in> yahalom
-      ==> Key K \<notin> analz (knows Spy evs) -->
+      \<Longrightarrow> Key K \<notin> analz (knows Spy evs) -->
           K \<in> symKeys -->
           Crypt K (Nonce NB) \<in> parts (knows Spy evs) -->
           Crypt (shrK B) \<lbrace>Agent A, Agent B, Key K, Nonce NB\<rbrace>
@@ -404,14 +400,12 @@ lemma Auth_A_to_B_lemma [rule_format]:
 apply (erule yahalom.induct, force,
        frule_tac [6] YM4_parts_knows_Spy)
 apply (analz_mono_contra, simp_all)
-txt\<open>Fake\<close>
-apply blast
-txt\<open>YM3: by \<open>new_keys_not_used\<close>, the message
-   @{term "Crypt K (Nonce NB)"} could not exist\<close>
-apply (force dest!: Crypt_imp_keysFor)
-txt\<open>YM4: was   @{term "Crypt K (Nonce NB)"} the very last message?  If so, 
-    apply unicity of session keys; if not, use the induction hypothesis\<close>
-apply (blast dest!: B_trusts_YM4_shrK dest: secure_unique_session_keys)
+  subgoal --\<open>Fake\<close> by blast
+  subgoal --\<open>YM3 because the message @{term "Crypt K (Nonce NB)"} could not exist\<close>
+    by (force dest!: Crypt_imp_keysFor)
+  subgoal --\<open>YM4: was @{term "Crypt K (Nonce NB)"} the very last message? If not, use the induction hypothesis,
+             otherwise by unicity of session keys\<close>
+    by (blast dest!: B_trusts_YM4_shrK dest: secure_unique_session_keys)
 done
 
 
@@ -419,11 +413,11 @@ text\<open>If B receives YM4 then A has used nonce NB (and therefore is alive).
   Moreover, A associates K with NB (thus is talking about the same run).
   Other premises guarantee secrecy of K.\<close>
 theorem YM4_imp_A_Said_YM3 [rule_format]:
-     "[| Gets B \<lbrace>Crypt (shrK B) \<lbrace>Agent A, Agent B, Key K, Nonce NB\<rbrace>,
+     "\<lbrakk>Gets B \<lbrace>Crypt (shrK B) \<lbrace>Agent A, Agent B, Key K, Nonce NB\<rbrace>,
                   Crypt K (Nonce NB)\<rbrace> \<in> set evs;
          (\<forall>NA. Notes Spy \<lbrace>Nonce NA, Nonce NB, Key K\<rbrace> \<notin> set evs);
-         K \<in> symKeys;  A \<notin> bad;  B \<notin> bad;  evs \<in> yahalom |]
-      ==> \<exists>X. Says A B \<lbrace>X, Crypt K (Nonce NB)\<rbrace> \<in> set evs"
+         K \<in> symKeys;  A \<notin> bad;  B \<notin> bad;  evs \<in> yahalom\<rbrakk>
+      \<Longrightarrow> \<exists>X. Says A B \<lbrace>X, Crypt K (Nonce NB)\<rbrace> \<in> set evs"
 by (blast intro: Auth_A_to_B_lemma
           dest: Spy_not_see_encrypted_key B_trusts_YM4_shrK)
 
